Add join target readiness to workload acceptance
Introduce EvJoinTargetReady as a state-neutral common event and add LkJoinTargetReady to the Awkernel workload task-trace family.

Track ready join targets separately from completed tasks so JoinWait dependencies are discharged by readiness observations rather than by terminal Complete events.

Regenerate the extracted Haskell workload checker and update the workload plan to describe the new readiness artifact.

extracted/haskell/AwkernelWorkloadAcceptance.hs
@@ -199,6 +199,7 @@ data OpEvent =
    EvWakeup JobId
  | EvBlock JobId
  | EvComplete JobId
+ | EvJoinTargetReady JobId
  | EvRequestResched CPU
  | EvHandleResched CPU
  | EvChoose CPU JobId
@@ -301,6 +302,7 @@ data AwkernelTaskTraceKind =
  | LkDispatch
  | LkSleep
  | LkJoinWait
+ | LkJoinTargetReady
  | LkComplete
 
 data AwkernelTaskTraceEntry =
@@ -379,19 +381,19 @@ add_pair_once x xs =
    True -> xs;
    False -> Cons x xs}
 
-all_dependencies_completed :: JobId -> (List (Prod JobId JobId)) -> (List
-                              JobId) -> Bool
-all_dependencies_completed task_id deps completed =
+all_dependencies_ready :: JobId -> (List (Prod JobId JobId)) -> (List
+                          JobId) -> Bool
+all_dependencies_ready task_id deps ready_targets =
   case deps of {
    Nil -> True;
    Cons p deps' ->
     case p of {
-     Pair waiter child ->
+     Pair waiter target ->
       case eqb0 waiter task_id of {
        True ->
-        andb (job_list_contains child completed)
-          (all_dependencies_completed task_id deps' completed);
-       False -> all_dependencies_completed task_id deps' completed}}}
+        andb (job_list_contains target ready_targets)
+          (all_dependencies_ready task_id deps' ready_targets);
+       False -> all_dependencies_ready task_id deps' ready_targets}}}
 
 bool_of_option_none :: (Option JobId) -> Bool
 bool_of_option_none oj =
@@ -423,6 +425,13 @@ sched_trace_event_is_complete :: JobId -> AwkernelSchedTraceEntry -> Bool
 sched_trace_event_is_complete j entry =
   case aste_event entry of {
    EvComplete j' -> eqb0 j' j;
+   _ -> False}
+
+sched_trace_event_is_join_target_ready :: JobId -> AwkernelSchedTraceEntry ->
+                                          Bool
+sched_trace_event_is_join_target_ready j entry =
+  case aste_event entry of {
+   EvJoinTargetReady j' -> eqb0 j' j;
    _ -> False}
 
 sched_trace_event_is_stutter :: AwkernelSchedTraceEntry -> Bool
@@ -477,6 +486,11 @@ sched_trace_is_complete j entry =
       (eqb (sched_trace_primary_need_resched entry) True))
     (bool_of_option_none (sched_trace_primary_dispatch_target entry))
 
+sched_trace_is_join_target_ready :: JobId -> AwkernelSchedTraceEntry -> Bool
+sched_trace_is_join_target_ready j entry =
+  andb (eqb0 (aste_cpu entry) (S O))
+    (sched_trace_event_is_join_target_ready j entry)
+
 sched_trace_is_stutter :: AwkernelSchedTraceEntry -> Bool
 sched_trace_is_stutter entry =
   andb
@@ -489,26 +503,33 @@ sched_trace_is_stutter entry =
 data AwkernelTaskTraceSummary =
    MkAwkernelTaskTraceSummary (Option JobId) (List JobId) (List
                                                           (Prod JobId JobId))
+ (List JobId)
 
 atts_root_task :: AwkernelTaskTraceSummary -> Option JobId
 atts_root_task a =
   case a of {
-   MkAwkernelTaskTraceSummary atts_root_task0 _ _ -> atts_root_task0}
+   MkAwkernelTaskTraceSummary atts_root_task0 _ _ _ -> atts_root_task0}
 
 atts_known_tasks :: AwkernelTaskTraceSummary -> List JobId
 atts_known_tasks a =
   case a of {
-   MkAwkernelTaskTraceSummary _ atts_known_tasks0 _ -> atts_known_tasks0}
+   MkAwkernelTaskTraceSummary _ atts_known_tasks0 _ _ -> atts_known_tasks0}
 
 atts_completion_deps :: AwkernelTaskTraceSummary -> List (Prod JobId JobId)
 atts_completion_deps a =
   case a of {
-   MkAwkernelTaskTraceSummary _ _ atts_completion_deps0 ->
+   MkAwkernelTaskTraceSummary _ _ atts_completion_deps0 _ ->
     atts_completion_deps0}
+
+atts_ready_targets :: AwkernelTaskTraceSummary -> List JobId
+atts_ready_targets a =
+  case a of {
+   MkAwkernelTaskTraceSummary _ _ _ atts_ready_targets0 ->
+    atts_ready_targets0}
 
 initial_task_trace_summary :: AwkernelTaskTraceSummary
 initial_task_trace_summary =
-  MkAwkernelTaskTraceSummary None Nil Nil
+  MkAwkernelTaskTraceSummary None Nil Nil Nil
 
 task_trace_entry_valid :: AwkernelTaskTraceSummary -> AwkernelTaskTraceEntry
                           -> Bool
@@ -523,11 +544,20 @@ task_trace_entry_valid summary entry =
         None -> option_job_eqb (atts_root_task summary) None});
    LkJoinWait ->
     case atte_related entry of {
-     Some child ->
+     Some target ->
       andb
         (job_list_contains (atte_subject entry) (atts_known_tasks summary))
-        (job_list_contains child (atts_known_tasks summary));
+        (job_list_contains target (atts_known_tasks summary));
      None -> False};
+   LkJoinTargetReady ->
+    case atte_related entry of {
+     Some _ -> False;
+     None ->
+      andb
+        (job_list_contains (atte_subject entry) (atts_known_tasks summary))
+        (negb
+          (job_list_contains (atte_subject entry)
+            (atts_ready_targets summary)))};
    _ -> job_list_contains (atte_subject entry) (atts_known_tasks summary)}
 
 task_trace_entry_step :: AwkernelTaskTraceSummary -> AwkernelTaskTraceEntry
@@ -539,14 +569,18 @@ task_trace_entry_step summary entry =
       Some _ -> atts_root_task summary;
       None -> Some (atte_subject entry)})
     (add_job_once (atte_subject entry) (atts_known_tasks summary))
-    (atts_completion_deps summary);
+    (atts_completion_deps summary) (atts_ready_targets summary);
    LkJoinWait ->
     case atte_related entry of {
-     Some child -> MkAwkernelTaskTraceSummary (atts_root_task summary)
+     Some target -> MkAwkernelTaskTraceSummary (atts_root_task summary)
       (atts_known_tasks summary)
-      (add_pair_once (Pair (atte_subject entry) child)
-        (atts_completion_deps summary));
+      (add_pair_once (Pair (atte_subject entry) target)
+        (atts_completion_deps summary))
+      (atts_ready_targets summary);
      None -> summary};
+   LkJoinTargetReady -> MkAwkernelTaskTraceSummary (atts_root_task summary)
+    (atts_known_tasks summary) (atts_completion_deps summary)
+    (add_job_once (atte_subject entry) (atts_ready_targets summary));
    _ -> summary}
 
 summarize_task_trace :: AwkernelTaskTraceSummary -> (List
@@ -563,34 +597,41 @@ summarize_task_trace summary task_trace =
 
 data AwkernelSchedTraceAcceptanceState =
    MkAwkernelSchedTraceAcceptanceState Bool (Option JobId) (List JobId) 
- (List JobId)
+ (List JobId) (List JobId)
 
 astas_started :: AwkernelSchedTraceAcceptanceState -> Bool
 astas_started a =
   case a of {
-   MkAwkernelSchedTraceAcceptanceState astas_started0 _ _ _ -> astas_started0}
+   MkAwkernelSchedTraceAcceptanceState astas_started0 _ _ _ _ ->
+    astas_started0}
 
 astas_selected :: AwkernelSchedTraceAcceptanceState -> Option JobId
 astas_selected a =
   case a of {
-   MkAwkernelSchedTraceAcceptanceState _ astas_selected0 _ _ ->
+   MkAwkernelSchedTraceAcceptanceState _ astas_selected0 _ _ _ ->
     astas_selected0}
 
 astas_dispatched :: AwkernelSchedTraceAcceptanceState -> List JobId
 astas_dispatched a =
   case a of {
-   MkAwkernelSchedTraceAcceptanceState _ _ astas_dispatched0 _ ->
+   MkAwkernelSchedTraceAcceptanceState _ _ astas_dispatched0 _ _ ->
     astas_dispatched0}
 
 astas_completed :: AwkernelSchedTraceAcceptanceState -> List JobId
 astas_completed a =
   case a of {
-   MkAwkernelSchedTraceAcceptanceState _ _ _ astas_completed0 ->
+   MkAwkernelSchedTraceAcceptanceState _ _ _ astas_completed0 _ ->
     astas_completed0}
+
+astas_ready_targets :: AwkernelSchedTraceAcceptanceState -> List JobId
+astas_ready_targets a =
+  case a of {
+   MkAwkernelSchedTraceAcceptanceState _ _ _ _ astas_ready_targets0 ->
+    astas_ready_targets0}
 
 initial_sched_trace_acceptance_state :: AwkernelSchedTraceAcceptanceState
 initial_sched_trace_acceptance_state =
-  MkAwkernelSchedTraceAcceptanceState False None Nil Nil
+  MkAwkernelSchedTraceAcceptanceState False None Nil Nil Nil
 
 sched_trace_step_start :: AwkernelTaskTraceSummary -> AwkernelSchedTraceEntry
                           -> Option AwkernelSchedTraceAcceptanceState
@@ -598,7 +639,7 @@ sched_trace_step_start summary entry =
   case atts_root_task summary of {
    Some root ->
     case sched_trace_is_wakeup root entry of {
-     True -> Some (MkAwkernelSchedTraceAcceptanceState True None Nil Nil);
+     True -> Some (MkAwkernelSchedTraceAcceptanceState True None Nil Nil Nil);
      False -> None};
    None -> None}
 
@@ -609,6 +650,7 @@ sched_trace_step_after_start :: AwkernelTaskTraceSummary ->
 sched_trace_step_after_start summary st entry =
   let {known = atts_known_tasks summary} in
   let {deps = atts_completion_deps summary} in
+  let {ready_targets = atts_ready_targets summary} in
   let {
    try_wakeup_job = \j ->
     case andb
@@ -626,7 +668,7 @@ sched_trace_step_after_start summary st entry =
              (negb (job_list_contains j (astas_completed st))))
            (option_job_eqb (astas_selected st) None) of {
      True -> Some (MkAwkernelSchedTraceAcceptanceState True (Some j)
-      (astas_dispatched st) (astas_completed st));
+      (astas_dispatched st) (astas_completed st) (astas_ready_targets st));
      False -> None}}
   in
   let {
@@ -634,7 +676,21 @@ sched_trace_step_after_start summary st entry =
     case andb (sched_trace_is_dispatch j entry)
            (option_job_eqb (astas_selected st) (Some j)) of {
      True -> Some (MkAwkernelSchedTraceAcceptanceState True None
-      (add_job_once j (astas_dispatched st)) (astas_completed st));
+      (add_job_once j (astas_dispatched st)) (astas_completed st)
+      (astas_ready_targets st));
+     False -> None}}
+  in
+  let {
+   try_join_target_ready = \j ->
+    case andb
+           (andb
+             (andb (sched_trace_is_join_target_ready j entry)
+               (job_list_contains j known))
+             (job_list_contains j ready_targets))
+           (negb (job_list_contains j (astas_ready_targets st))) of {
+     True -> Some (MkAwkernelSchedTraceAcceptanceState True None
+      (astas_dispatched st) (astas_completed st)
+      (add_job_once j (astas_ready_targets st)));
      False -> None}}
   in
   let {
@@ -644,9 +700,10 @@ sched_trace_step_after_start summary st entry =
              (andb (sched_trace_is_complete j entry)
                (job_list_contains j (astas_dispatched st)))
              (negb (job_list_contains j (astas_completed st))))
-           (all_dependencies_completed j deps (astas_completed st)) of {
+           (all_dependencies_ready j deps (astas_ready_targets st)) of {
      True -> Some (MkAwkernelSchedTraceAcceptanceState True None
-      (astas_dispatched st) (add_job_once j (astas_completed st)));
+      (astas_dispatched st) (add_job_once j (astas_completed st))
+      (astas_ready_targets st));
      False -> None}}
   in
   case sched_trace_is_stutter entry of {
@@ -660,7 +717,10 @@ sched_trace_step_after_start summary st entry =
        None ->
         case first_some try_dispatch_job known of {
          Some st' -> Some st';
-         None -> first_some try_complete_job known}}}}
+         None ->
+          case first_some try_join_target_ready known of {
+           Some st' -> Some st';
+           None -> first_some try_complete_job known}}}}}
 
 sched_trace_step :: AwkernelTaskTraceSummary ->
                     AwkernelSchedTraceAcceptanceState ->
@@ -1014,4 +1074,3 @@ awk_workload_accepts_global_fifo_scheduler_relation_sched_trace task_trace sched
   andb (awk_workload_accepts_sched_trace task_trace sched_trace)
     (sched_trace_global_fifo_scheduler_relation_checkb task_trace
       sched_trace)
-
